"iRename select" equivalent tactic

src/Iris/ProofMode/Tactics/Rename.lean
@@ -6,13 +6,14 @@ Authors: Lars König, Mario Carneiro
 import Iris.BI
 import Iris.ProofMode.Expr
 import Iris.ProofMode.Classes
+import Iris.ProofMode.Tactics.Basic
 import Iris.Std
 import Lean.Elab
 
 namespace Iris.ProofMode
 open Lean Elab Tactic Qq
 
-variable (old new : Name) {prop : Q(Type)} {bi : Q(BI $prop)} in
+variable (old : Name → Name → Bool) (new : Name) {prop : Q(Type)} {bi : Q(BI $prop)} in
 def Hyps.rename : ∀ {e}, Hyps bi e → Option (Hyps bi e)
   | _, .emp _ => none
   | _, .sep _ _ _ _ lhs rhs =>
@@ -21,7 +22,8 @@ def Hyps.rename : ∀ {e}, Hyps bi e → Option (Hyps bi e)
     | none => match lhs.rename with
       | some lhs' => some (.mkSep lhs' rhs _)
       | none => none
-  | _, .hyp _ name uniq p ty _ => if old == name then some (Hyps.mkHyp bi new uniq p ty _) else none
+  | _, .hyp _ name uniq p ty _ =>
+    if old name uniq then some (Hyps.mkHyp bi new uniq p ty _) else none
 
 elab "irename" colGt nameFrom:ident " => " colGt nameTo:ident : tactic => do
   -- parse syntax
@@ -34,6 +36,23 @@ elab "irename" colGt nameFrom:ident " => " colGt nameTo:ident : tactic => do
   let g ← instantiateMVars <| ← mvar.getType
   let some { prop, bi, hyps, goal } := parseIrisGoal? g | throwError "not in proof mode"
 
-  let some hyps' := hyps.rename nameFrom.getId nameTo.getId | throwError "unknown hypothesis"
+  let some hyps' := hyps.rename (fun name _ => name == nameFrom.getId) nameTo.getId
+    | throwError "unknown hypothesis"
+
+  mvar.setType (IrisGoal.toExpr { prop, bi, hyps := hyps', goal })
+
+elab "irename" ":" colGt ty:term " => " colGt nameTo:ident : tactic => do
+  -- parse syntax
+  if nameTo.getId.isAnonymous then
+    throwUnsupportedSyntax
+
+  -- find hypothesis index
+  let mvar ← getMainGoal
+  mvar.withContext do
+  let g ← instantiateMVars <| ← mvar.getType
+  let some { prop, bi, hyps, goal } := parseIrisGoal? g | throwError "not in proof mode"
+
+  let uniq ← try selectHyp (← elabTerm ty prop) hyps catch _ => throwError "unknown hypothesis"
+  let some hyps' := hyps.rename (fun _ uniq' => uniq == uniq') nameTo.getId | unreachable!
 
   mvar.setType (IrisGoal.toExpr { prop, bi, hyps := hyps', goal })
